HeapLang/State.thy
@@ -4,38 +4,40 @@ begin
 
 section \<open> State \<close>
 text \<open> State specific definitions and lemmata; 
-       from https://gitlab.mpi-sws.org/iris/iris/-/blob/master/iris_heap_lang/lang.v \<close>
+  based on https://gitlab.mpi-sws.org/iris/iris/-/blob/master/iris_heap_lang/lang.v \<close>
 
 (* The state: heaps of val options, with None representing deallocated locations. *)
-datatype state = State (heap: "(loc,val) map") (used_proph_id: "proph_id set")
+datatype state = State (heap: "(loc,val option) map") (used_proph_id: "proph_id set")
 
-definition state_upd_heap :: "((loc,val) map \<Rightarrow> (loc,val) map) \<Rightarrow> state \<Rightarrow> state" where
+definition state_upd_heap :: "((loc,val option) map \<Rightarrow> (loc,val option) map) \<Rightarrow> state \<Rightarrow> state" where
   "state_upd_heap f \<sigma> = State (f (heap \<sigma>)) (used_proph_id \<sigma>)"
 
 definition state_upd_used_proph_id :: "(proph_id set \<Rightarrow> proph_id set) \<Rightarrow> state \<Rightarrow> state" where
   "state_upd_used_proph_id f \<sigma> = State (heap \<sigma>) (f (used_proph_id \<sigma>))"
 
-fun heap_array :: "loc \<Rightarrow> val list \<Rightarrow> (loc, val) map" where
+fun heap_array :: "loc \<Rightarrow> val list \<Rightarrow> (loc, val option) map" where
   "heap_array l [] = Map.empty"
-| "heap_array l (v#vs) = (heap_array (l+\<^sub>\<iota>1) vs)(l\<mapsto>v)"
+| "heap_array l (v#vs) = (heap_array (l+\<^sub>\<iota>1) vs)(l\<mapsto>Some v)"
   
-lemma heap_array_singleton: "heap_array l [v] = [l\<mapsto>v]" by simp
+lemma heap_array_singleton: "heap_array l [v] = [l\<mapsto>Some v]" by simp
 
-lemma heap_array_dom: "dom (heap_array l vs) = Loc ` {(loc_car l)..< (loc_car l) + int (length vs)}"
+lemma heap_array_dom: "dom (heap_array l vs) = {l..< (l +\<^sub>\<iota> int (length vs))}"
 proof (induction vs arbitrary: l)
   case (Cons a vs)
   have "dom (heap_array l (a # vs)) = insert l (dom (heap_array (l+\<^sub>\<iota>1) vs))" by simp
-  also have "... = insert l (Loc ` {(loc_car (l+\<^sub>\<iota>1))..< (loc_car (l+\<^sub>\<iota>1)) + int (length vs)})" 
+  also have "... = insert l {(l+\<^sub>\<iota>1)..< ((l+\<^sub>\<iota>1) +\<^sub>\<iota> int (length vs))}" 
     using Cons by simp
-  also have "... = Loc ` ({loc_car l} \<union> {(loc_car (l+\<^sub>\<iota>1))..< (loc_car (l+\<^sub>\<iota>1)) + int (length vs)})" 
+  also have "... = {l} \<union> {(l+\<^sub>\<iota>1)..< ((l+\<^sub>\<iota>1) +\<^sub>\<iota> int (length vs))}" 
       by simp
-  also have "... = Loc ` ({(loc_car l)..<(loc_car (l+\<^sub>\<iota>1))} \<union>
-    {(loc_car (l+\<^sub>\<iota>1))..< (loc_car (l+\<^sub>\<iota>1)) + int (length vs)})" using loc_add_def by force
-  also have "... = Loc ` ({(loc_car l)..<(loc_car l)+1} \<union>
-    {(loc_car l)+1..< (loc_car l) + 1 + int (length vs)})" by (simp add: loc_add_def) 
-  also have "... = Loc ` {(loc_car l)..< (loc_car l) + int (length (a#vs))}" by auto
+  also have "... = ({l..<(l+\<^sub>\<iota>1)} \<union>
+    {(l+\<^sub>\<iota>1)..<((l+\<^sub>\<iota>1) +\<^sub>\<iota> int (length vs))})" using less_eq_loc_def loc_add_def less_loc_def loc.expand
+    by fastforce
+  also have "... = ({l..<(l+\<^sub>\<iota>1)} \<union> {(l+\<^sub>\<iota>1)..<(l+\<^sub>\<iota>(1 + int (length vs)))})" by (simp add: loc_add_assoc)
+  also have "... = ({l..<(l+\<^sub>\<iota>1)} \<union> {(l+\<^sub>\<iota>1)..<(l+\<^sub>\<iota> int (length (a#vs)))})" by simp
+  also have "... = {l..<(l +\<^sub>\<iota> int (length (a#vs)))}" 
+    by (auto simp: loc_add_def loc.expand less_eq_loc_def ivl_disj_un(17))
   finally show ?case .
-qed (simp)
+qed (simp add: loc_add_0)
 
 lemma heap_array_shift: "heap_array l vs k = heap_array (l+\<^sub>\<iota>n) vs (k+\<^sub>\<iota>n)"
 proof (induction vs arbitrary: l k)
@@ -48,12 +50,12 @@ lemma heap_array_cons_shift: "(heap_array l vs k = Some w) \<Longrightarrow> (he
 proof -
   assume assm: "heap_array l vs k = Some w"
   hence "k \<in> dom (heap_array l vs)" by blast
-  with heap_array_dom[of l vs] have "l\<noteq>k+\<^sub>\<iota>1" using loc_add_def by auto
+  with heap_array_dom[of l vs] have "l\<noteq>k+\<^sub>\<iota>1" using loc_add_def less_eq_loc_def by auto
   with assm show "heap_array l (v#vs) (k+\<^sub>\<iota>1) = Some w" unfolding loc_add_def apply auto 
   using heap_array_shift loc_add_def by fastforce
 qed
 
-lemma heap_array_elements: "heap_array l vs k = Some w \<Longrightarrow> w \<in> set vs"
+lemma heap_array_elements: "heap_array l vs k = Some (Some w) \<Longrightarrow> w \<in> set vs"
 proof (induction vs arbitrary: l k)
   case (Cons a vs)
   then show ?case by (metis fun_upd_apply heap_array.simps(2) in_set_member member_rec(1) option.inject)
@@ -66,7 +68,7 @@ proof (induction vs arbitrary: l k v)
   with Cons(2) have step: "heap_array (l+\<^sub>\<iota>1) (a#vs) k = Some w" by simp
   then show ?case proof (cases "(l+\<^sub>\<iota>1=k)")
     case True
-    with step have "w=a" by simp
+    with step have "w=Some a" by simp
     with True show ?thesis unfolding loc_add_def by auto
   next
     case False
@@ -77,13 +79,13 @@ proof (induction vs arbitrary: l k v)
 qed (simp)
 
 (* Due to nth being defined as primrec, this can't be an iff but only a one sided implication. *)
-lemma heap_array_lookup: "((heap_array l vs) k = Some ow) \<Longrightarrow>
+lemma heap_array_lookup: "((heap_array l vs) k = Some (Some ow)) \<Longrightarrow>
   (\<exists>j w. 0 \<le> j \<and> k = l +\<^sub>\<iota> j \<and> vs!(nat j) = w \<and> w=ow)"
 proof (induction vs arbitrary: k)
   case (Cons a vs)
   then show ?case proof (cases "l=k")
     case True
-    hence "heap_array l (a#vs) k = Some a" by simp
+    hence "heap_array l (a#vs) k = Some (Some a)" by simp
     with Cons(2) have "ow = a" by simp
     moreover from True have "k=l+\<^sub>\<iota>0 \<and> (0::int)\<le>0 \<and> (a#vs)!(nat 0) = a" by (simp add: loc_add_0)
     ultimately show ?thesis by blast
@@ -102,8 +104,125 @@ lemma state_array_map_disjoint: "(\<forall>i. (0\<le>i \<longrightarrow> (nat i 
 proof
   assume assm: "\<forall>i\<ge>0. nat i < length vs \<longrightarrow> h (l +\<^sub>\<iota> i) = None"
   from assm have "\<forall>i\<ge>0. nat i < length vs \<longrightarrow> (l +\<^sub>\<iota> i) \<notin> dom h" by fastforce
-  with heap_array_dom have "\<forall>k\<in>dom (heap_array l vs). k \<notin> dom h"
-  by (smt (verit, best) atLeastLessThan_iff domD heap_array_lookup imageE loc.inject loc_add_def nat_less_iff)
-  then show "dom (heap_array l vs) \<inter> dom h \<subseteq> {}" by auto
+  hence "\<forall>i \<in> {0..<(int (length vs))}. (l +\<^sub>\<iota> i) \<notin> dom h" by fastforce
+  hence "\<forall>l' \<in> {(l +\<^sub>\<iota> i) | i. i \<in> {0..<(int (length vs))} }. l' \<notin> dom h" by blast
+  hence "\<forall>l' \<in> {l..<(l +\<^sub>\<iota> int (length vs))}. l' \<notin> dom h" using loc_ranges by blast
+  hence "{l..<(l +\<^sub>\<iota> int (length vs))} \<inter> dom h = {}" by auto
+  with heap_array_dom show "dom (heap_array l vs) \<inter> dom h \<subseteq> {}" by auto
 qed (simp)
+
+definition state_init_heap :: "loc \<Rightarrow> nat \<Rightarrow> val \<Rightarrow> state \<Rightarrow> state" where
+  "state_init_heap l n v \<sigma> = state_upd_heap (\<lambda>h. h ++ heap_array l (replicate n v)) \<sigma>"
+
+lemma state_init_heap_singleton: "state_init_heap l 1 v \<sigma> = state_upd_heap (\<lambda>h. h(l\<mapsto>Some v)) \<sigma>"
+unfolding state_init_heap_def by simp
+
+inductive head_step :: "expr \<Rightarrow> state \<Rightarrow> observation list \<Rightarrow> expr \<Rightarrow> state \<Rightarrow> expr list \<Rightarrow> bool" 
+  ("_ _ _ \<Rightarrow>\<^sub>h _ _ _")  where
+  RecS: "(Rec f x e) \<sigma> [] \<Rightarrow>\<^sub>h (Val(RecV f x e)) \<sigma> []"
+| PairS: "(Pair (Val v1) (Val v2)) \<sigma> [] \<Rightarrow>\<^sub>h (Val(PairV v1 v2)) \<sigma> []"
+| InjLS: "(InjL(Val v)) \<sigma> [] \<Rightarrow>\<^sub>h (Val(InjLV v)) \<sigma> []"
+| InjRS: "(InjR(Val v)) \<sigma> [] \<Rightarrow>\<^sub>h (Val(InjRV v)) \<sigma> []"
+| BetaS: "e' = subst' x v2 (subst' f (RecV f x e1) e1) \<Longrightarrow>
+  (App (Val(RecV f x e1)) (Val v2)) \<sigma> [] \<Rightarrow>\<^sub>h e' \<sigma> []"
+| UnOpS: "un_op_eval op v = Some v' \<Longrightarrow>
+  (UnOp op (Val v)) \<sigma> [] \<Rightarrow>\<^sub>h (Val v') \<sigma> []"
+| BinOpS: "bin_op_eval op v1 v2 = Some v' \<Longrightarrow>
+  (BinOp op (Val v1) (Val v2)) \<sigma> [] \<Rightarrow>\<^sub>h (Val v') \<sigma> []"
+| IfTrueS: "(If (Val(LitV(LitBool True))) e1 e2) \<sigma> [] \<Rightarrow>\<^sub>h e1 \<sigma> []"
+| IfFalseS: "(If (Val(LitV(LitBool False))) e1 e2) \<sigma> [] \<Rightarrow>\<^sub>h e2 \<sigma> []"
+| FstS: "(Fst (Val(PairV v1 v2))) \<sigma> [] \<Rightarrow>\<^sub>h (Val v1) \<sigma> []"
+| SndS: "(Snd (Val(PairV v1 v2))) \<sigma> [] \<Rightarrow>\<^sub>h (Val v2) \<sigma> []"
+| CaseLS: "(Case (Val(InjLV v)) e1 e2) \<sigma> [] \<Rightarrow>\<^sub>h (App e1 (Val v)) \<sigma> []"
+| CaseRS: "(Case (Val(InjRV v)) e1 e2) \<sigma> [] \<Rightarrow>\<^sub>h (App e2 (Val v)) \<sigma> []"
+| ForkS: "(Fork e) \<sigma> [] \<Rightarrow>\<^sub>h (Val(LitV LitUnit)) \<sigma> [e]"
+| AllocNS: "\<lbrakk>(0 < n); (\<forall> (i::int). (0 \<le> i) \<Longrightarrow> (i < n) \<Longrightarrow> heap \<sigma> (l +\<^sub>\<iota> i) = None)\<rbrakk> \<Longrightarrow>
+  (AllocN (Val(LitV(LitInt n))) (Val v)) \<sigma> [] \<Rightarrow>\<^sub>h
+  (Val(LitV(LitLoc l))) (state_init_heap l (nat n) v \<sigma>) []"
+| FreeS: "heap \<sigma> l = Some v \<Longrightarrow> 
+  (Free (Val(LitV(LitLoc l)))) \<sigma> [] \<Rightarrow>\<^sub>h (Val(LitV LitUnit)) (state_upd_heap (\<lambda>h. h(l\<mapsto>None)) \<sigma>) []"
+| LoadS: "heap \<sigma> l = Some (Some v) \<Longrightarrow> (Load (Val(LitV(LitLoc l)))) \<sigma> [] \<Rightarrow>\<^sub>h (of_val v) \<sigma> []"
+| StoreS: "heap \<sigma> l = Some (Some v) \<Longrightarrow>
+  (Store (Val(LitV(LitLoc l))) (Val w)) \<sigma> [] \<Rightarrow>\<^sub>h
+  (Val(LitV LitUnit)) (state_upd_heap (\<lambda>h. h(l\<mapsto>Some w)) \<sigma>) []"
+| XchgS: "heap \<sigma> l = Some (Some v1) \<Longrightarrow>
+  (Xchg (Val(LitV(LitLoc l))) (Val v2)) \<sigma> [] \<Rightarrow>\<^sub>h
+  (Val v1) (state_upd_heap (\<lambda>h. h(l\<mapsto>Some v2)) \<sigma>) []"
+   (* Crucially, this compares the same way as [EqOp]! *)
+| CmpXchgS: "\<lbrakk>heap \<sigma> l = Some (Some vl); vals_compare_safe vl v1; b = (vl = v1)\<rbrakk> \<Longrightarrow>
+  (CmpXchg (Val(LitV(LitLoc l))) (Val v1) (Val v2)) \<sigma> [] \<Rightarrow>\<^sub>h
+  (Val(PairV vl (LitV(LitBool b)))) (if b then state_upd_heap (\<lambda>h. h(l\<mapsto>Some v2)) \<sigma> else \<sigma>) []"
+| FaaS: "heap \<sigma> l = Some (Some (LitV (LitInt i1))) \<Longrightarrow>
+  (FAA (Val(LitV(LitLoc l))) (Val(LitV(LitInt i2)))) \<sigma> [] \<Rightarrow>\<^sub>h
+  (Val(LitV(LitInt i1))) (state_upd_heap (\<lambda>h. h(l\<mapsto>Some (LitV (LitInt (i1 + i2))))) \<sigma>) []"
+| NewProphS: "p \<notin> used_proph_id \<sigma> \<Longrightarrow>
+  NewProph \<sigma> [] \<Rightarrow>\<^sub>h (Val(LitV(LitProphecy p))) (state_upd_used_proph_id (insert p) \<sigma>) []"
+| ResolveS: "e \<sigma> \<kappa>s \<Rightarrow>\<^sub>h (Val v) \<sigma>' ts \<Longrightarrow>
+  (Resolve e (Val(LitV(LitProphecy p))) (Val w)) \<sigma> (\<kappa>s@[(p, (v, w))]) \<Rightarrow>\<^sub>h (Val v) \<sigma>' ts"
+ 
+declare head_step.intros[intro]
+inductive_cases headE[elim]: "(Rec f x e) \<sigma> \<kappa> \<Rightarrow>\<^sub>h e2 \<sigma>2 \<kappa>2"
+  "(Pair v1 v2) \<sigma> \<kappa> \<Rightarrow>\<^sub>h e2 \<sigma>2 \<kappa>2"
+  "(InjL v) \<sigma> \<kappa> \<Rightarrow>\<^sub>h e2 \<sigma>2 \<kappa>2"
+  "(InjR v) \<sigma> \<kappa> \<Rightarrow>\<^sub>h e2 \<sigma>2 \<kappa>2"
+  "(App f v2) \<sigma> \<kappa> \<Rightarrow>\<^sub>h e' \<sigma>2 \<kappa>2"
+  "(UnOp op v) \<sigma> \<kappa> \<Rightarrow>\<^sub>h e2 \<sigma>2 \<kappa>2"
+  "(BinOp op v1 v2) \<sigma> \<kappa> \<Rightarrow>\<^sub>h e2 \<sigma>2 \<kappa>2"
+  "(If b e1 e2) \<sigma> \<kappa> \<Rightarrow>\<^sub>h e' \<sigma>2 \<kappa>2"
+  "(Fst v) \<sigma> \<kappa> \<Rightarrow>\<^sub>h e2 \<sigma>2 \<kappa>2"
+  "(Snd v) \<sigma> \<kappa> \<Rightarrow>\<^sub>h e2 \<sigma>2 \<kappa>2"
+  "(Case v e1 e2) \<sigma> \<kappa> \<Rightarrow>\<^sub>h e2 \<sigma>2 \<kappa>2"
+  "(Fork e) \<sigma> \<kappa> \<Rightarrow>\<^sub>h e2 \<sigma>2 efs"
+  "(AllocN e v) \<sigma> \<kappa> \<Rightarrow>\<^sub>h e2 \<sigma>2 \<kappa>2"
+  "(Free l) \<sigma> \<kappa> \<Rightarrow>\<^sub>h e2 \<sigma>2 \<kappa>2"
+  "(Load l) \<sigma> \<kappa> \<Rightarrow>\<^sub>h e2 \<sigma>2 \<kappa>2"
+  "(Store l v) \<sigma> \<kappa> \<Rightarrow>\<^sub>h e2 \<sigma>2 \<kappa>2"
+  "(Xchg l v) \<sigma> \<kappa> \<Rightarrow>\<^sub>h e2 \<sigma>2 \<kappa>2"
+  "(CmpXchg l v1 v2) \<sigma> \<kappa> \<Rightarrow>\<^sub>h e2 \<sigma>2 \<kappa>2"
+  "(FAA l i) \<sigma> \<kappa> \<Rightarrow>\<^sub>h e2 \<sigma>2 \<kappa>2"
+  "NewProph \<sigma> \<kappa> \<Rightarrow>\<^sub>h e2 \<sigma>2 \<kappa>2"
+  "(Resolve e (Val v1) (Val w)) \<sigma> \<kappa> \<Rightarrow>\<^sub>h e2 \<sigma>2 \<kappa>2"
+  
+lemma fill_item_val: "\<exists>x. Some x = (to_val (fill_item Ki e)) \<Longrightarrow> \<exists>x. Some x = (to_val e)"
+by (induct Ki) auto
+
+lemma val_head_stuck: "(e1 \<sigma>1 \<kappa> \<Rightarrow>\<^sub>h e2 \<sigma>2 efs) \<Longrightarrow> (to_val e1 = None)"
+by (induct rule: head_step.induct) auto
+
+lemma head_ctx_step_val: "(fill_item Ki e) \<sigma>1 \<kappa> \<Rightarrow>\<^sub>h e2 \<sigma>2 efs \<Longrightarrow> \<exists>x. Some x = (to_val e)"
+proof (induction Ki arbitrary: \<kappa> e2)
+  case (CaseCtx x1a x2a)
+  then show ?case by cases auto
+next
+  case (ResolveLCtx Ki v1 v2)
+  hence step: "(Resolve (fill_item Ki e) (Val v1) (Val v2)) \<sigma>1 \<kappa> \<Rightarrow>\<^sub>h e2 \<sigma>2 efs" by simp
+  show ?case by (rule headE(21)[OF step, of "\<exists>x. Some x = to_val e"]) (simp add: ResolveLCtx(1))
+next
+  case (ResolveMCtx x1a x2a)
+  then show ?case by cases auto
+next
+  case (ResolveRCtx x1a x2a)
+  then show ?case by cases auto
+qed auto
+ 
+lemma fill_item_no_val_inj: "\<lbrakk>to_val e1 = None; to_val e2 = None; fill_item Ki1 e1 = fill_item Ki2 e2\<rbrakk>
+   \<Longrightarrow> Ki1 = Ki2"
+proof (induction Ki2)
+  case (ResolveLCtx Ki2 x2a x3a)
+  show ?case using ResolveLCtx proof (induction Ki1)
+    case (ResolveLCtx Ki1 x2a x3a)
+    then show ?case sorry (* I have no idea how/why this works in Coq. *)
+  qed auto
+qed (induction Ki1; auto)+
+
+lemma alloc_fresh:  "(0 < n) \<Longrightarrow>
+  (AllocN ((Val(LitV(LitInt n)))) (Val v)) \<sigma> [] \<Rightarrow>\<^sub>h
+  (Val(LitV(LitLoc (fresh_locs (F (dom (heap \<sigma>))))))) (state_init_heap (fresh_locs (F (dom (heap \<sigma>)))) (nat n) v \<sigma>) []"
+by blast
+
+lemma head_step_to_val: "\<lbrakk>e1 \<sigma>1 \<kappa> \<Rightarrow>\<^sub>h e2 \<sigma>2 efs; e1 \<sigma>1' \<kappa>' \<Rightarrow>\<^sub>h e2' \<sigma>2' efs'; \<exists>x. Some x = (to_val e2)\<rbrakk>
+  \<Longrightarrow> \<exists>x. Some x = (to_val e2')"
+  by (induction rule: head_step.induct) auto
+
+(* Other lemmata contain references to the Iris base logic and can thus not be defined yet. *)
 end
