README.md
@@ -1,1 +1,6 @@
-TBD
+# IsarIris
+
+This is an experimental/partial port of the [Iris](https://gitlab.mpi-sws.org/iris/iris) separation logic framework to Isabelle/HOL.
+We focus on the HeapLang formalization and investigate the differences in automating reasoning in the Iris logic based on on this.
+
+This work is conducted as part of a master thesis project and will thus be developed solely by the author until the thesis work is done.
